making preamble an index

pulse/src/ocaml/plugin/generated/Pulse_Checker_Auto_IntroRewrite.ml
@@ -1,7 +1,8 @@
 open Prims
 let (intro_rewrite : Pulse_Checker_Auto_Util.intro_from_unmatched_fn) =
   fun g ->
-    fun p ->
-      Obj.magic
-        (FStar_Tactics_Effect.lift_div_tac
-           (fun uu___ -> FStar_Pervasives_Native.None))
+    fun uu___ ->
+      fun p ->
+        Obj.magic
+          (FStar_Tactics_Effect.lift_div_tac
+             (fun uu___1 -> FStar_Pervasives_Native.None))
